proof/invariant-abstract/ARM/ArchVSpaceEntries_AI.thy
@@ -695,8 +695,12 @@ crunch valid_pdpt_objs[wp]: test_possible_switch_to "valid_pdpt_objs"
 crunch valid_pdpt_objs[wp]: reorder_ntfn, reorder_ep, thread_set_priority, set_priority "valid_pdpt_objs"
   (wp: crunch_wps simp: crunch_simps)
 
+crunch valid_pdpt_objs[wp]: invoke_domain "valid_pdpt_objs::det_state \<Rightarrow> _"
+  (wp: check_cap_inv hoare_vcg_if_lift2 simp: crunch_simps
+       ignore: check_cap_at set_object tcb_release_enqueue test_possible_switch_to)
+
 crunch valid_pdpt_objs[wp]: invoke_tcb, invoke_domain "valid_pdpt_objs::det_state \<Rightarrow> _"
-  (wp: check_cap_inv crunch_wps simp: crunch_simps
+  (wp: check_cap_inv crunch_wps hoare_vcg_if_lift2 simp: crunch_simps
        ignore: check_cap_at set_object tcb_release_enqueue test_possible_switch_to)
 
 crunch valid_pdpt_objs[wp]: invoke_irq_handler "valid_pdpt_objs"
