proof/invariant-abstract/CSpaceInv_AI.thy
@@ -2031,6 +2031,7 @@ lemma cap_insert_objs [wp]:
 
 crunches cap_insert, set_cdt
   for pred_tcb_at[wp]: "\<lambda>s. Q (pred_tcb_at proj P t s)"
+  and sc_at_pred_n[wp]: "\<lambda>s. Q (sc_at_pred_n N proj P p s)"
   and ct [wp]: "\<lambda>s. P (cur_thread s)"
   and cur_sc [wp]: "\<lambda>s. P (cur_sc s)"
   and ct_in_state[wp]: "ct_in_state P"
